showing secrecy property for Online protocol - init

dy-extensions/DY.Simplified.fst
@@ -4,6 +4,8 @@ open Comparse
 open DY.Core
 open DY.Lib
 
+#set-options "--fuel 0 --ifuel 1 --z3rlimit 25  --z3cliopt 'smt.qi.eager_threshold=100'"
+
 val start_new_session:
   #a:Type -> {| local_state a |} ->
   principal -> a ->
@@ -21,8 +23,42 @@ val pk_enc_for:
   traceful (option bytes)
 let pk_enc_for #a alice bob key_sid key_tag plaintext =
   let*? pk_bob = get_public_key alice key_sid (LongTermPkEncKey key_tag) bob in
-  let* nonce = mk_rand PkNonce (principal_label bob) 32 in
+  let* nonce = mk_rand PkNonce (principal_label alice) 32 in
   return ( Some (pk_enc pk_bob nonce (serialize a plaintext)))
+
+val bytes_invariant_pk_enc_for:
+  {|protocol_invariants|}->
+  tr:trace ->
+  #a:Type -> {|parseable_serializeable bytes a|} ->
+  alice:principal -> bob:principal ->
+  alice_pki_sid:state_id ->
+  key_tag:string ->
+  msg:a ->
+  Lemma
+  (requires
+      trace_invariant tr
+    /\ has_pki_invariant
+    /\ is_knowable_by ( principal_label alice `join` principal_label bob ) tr (serialize a msg)
+    /\ pkenc_pred.pred tr (long_term_key_type_to_usage (LongTermPkEncKey key_tag) bob) (serialize a msg)
+  )
+  (ensures (
+    match pk_enc_for alice bob alice_pki_sid key_tag msg tr with
+    | (None, _) -> True
+    | (Some cipher, tr_out) -> 
+        is_publishable tr_out cipher
+  ))
+let bytes_invariant_pk_enc_for #pinvs tr #a alice bob alice_pki_sid key_tag msg =
+  match pk_enc_for alice bob alice_pki_sid key_tag msg tr with
+  | (None, _) -> ()
+  | (Some cipher, tr_out) -> (
+      let pk_type = LongTermPkEncKey key_tag in
+      let (Some pk_bob, _) = get_public_key alice alice_pki_sid pk_type bob tr in
+      let (nonce, tr_nonce) = mk_rand PkNonce (principal_label alice) 32 tr in
+      let msg = serialize #bytes a msg in
+      assert(is_public_key_for tr_out pk_bob pk_type bob);
+      let sk_usg = long_term_key_type_to_usage (LongTermPkEncKey key_tag) bob in
+      pkenc_pred.pred_later tr tr_out sk_usg msg
+)  
 
 val pk_dec_with_key_lookup:
   #a:Type -> {| parseable_serializeable bytes a |} ->
