examples/Online_with_secrecy/DY.OnlineS.Invariants.Proofs.fst
@@ -1,0 +1,40 @@
+module DY.OnlineS.Invariants.Proofs
+
+open Comparse
+open DY.Core
+open DY.Lib
+
+open DY.Simplified
+
+open DY.OnlineS.Protocol
+open DY.OnlineS.Invariants
+
+#set-options "--fuel 0 --ifuel 1 --z3rlimit 25  --z3cliopt 'smt.qi.eager_threshold=100'"
+
+val send_ping_invariant:
+  alice:principal -> bob:principal -> keys_sid:state_id ->
+  tr:trace ->
+  Lemma
+  ( requires trace_invariant tr
+  )
+  (ensures (
+    let (_ , tr_out) = send_ping alice bob keys_sid tr in
+    trace_invariant tr_out
+  ))
+let send_ping_invariant alice bob keys_sid  tr =
+  let (n_a, tr_rand) = mk_rand NoUsage (nonce_label alice bob) 32 tr in
+  assert(trace_invariant tr_rand);
+
+  let ping = Ping {p_alice = alice; p_n_a = n_a} in 
+  match pk_enc_for alice bob keys_sid key_tag ping tr_rand with
+  | (None, _) -> ()
+  | (Some ping_encrypted, tr_enc) -> (
+      assert(trace_invariant tr_enc);
+      let (msg_ts, tr_msg) = send_msg ping_encrypted tr_enc in
+      serialize_wf_lemma message (is_knowable_by (nonce_label alice bob) tr_rand) ping;
+      bytes_invariant_pk_enc_for tr_rand alice bob keys_sid key_tag ping;
+      assert(trace_invariant tr_msg);
+      let st = SentPing {sp_bob = bob; sp_n_a = n_a} in
+      let (sid, tr_sess) = start_new_session alice st tr_msg in
+      assert(trace_invariant tr_sess)
+  )
