examples/Online_with_secrecy/DY.OnlineS.Tmp.fst
@@ -1,0 +1,64 @@
+module DY.OnlineS.Tmp
+
+open Comparse
+open DY.Core
+open DY.Lib
+
+#set-options "--fuel 0 --ifuel 1 --z3rlimit 25  --z3cliopt 'smt.qi.eager_threshold=100'"
+
+[@@ with_bytes bytes]
+type cont_t = {
+  p: principal;
+  n: bytes
+}
+
+[@@ with_bytes bytes]
+type state = 
+ | S: cont_t -> state
+ | S2: principal -> bytes -> state
+
+%splice [ps_cont_t] (gen_parser (`cont_t))
+%splice [ps_cont_t_is_well_formed] (gen_is_well_formed_lemma (`cont_t))
+
+
+%splice [ps_state] (gen_parser (`state))
+%splice [ps_state_is_well_formed] (gen_is_well_formed_lemma (`state))
+
+instance parseable_serializeable_bytes_state: parseable_serializeable bytes state = mk_parseable_serializeable ps_state
+
+instance local_state_state: local_state state = {
+  tag = "S";
+  format = parseable_serializeable_bytes_state;
+}
+
+instance crypto_usages_p : crypto_usages = default_crypto_usages
+
+let crypto_p : crypto_predicates = { 
+  default_crypto_predicates with 
+  pkenc_pred = { 
+    pred = (fun tr sk_usage msg -> True); 
+    pred_later = (fun tr1 tr2 pk msg -> ()) 
+  } 
+}
+
+instance crypto_invariants_p: crypto_invariants = {
+  usages = crypto_usages_p;
+  preds =  crypto_p
+}
+
+let state_predicate_nsl: local_state_predicate state = {
+  pred = (fun tr prin sess_id st ->
+    match st with
+    | S cont -> 
+        is_knowable_by (principal_label prin) tr cont.n
+    | S2 _ n ->    
+        is_knowable_by (principal_label prin) tr n
+  );
+  pred_later = (fun tr1 tr2 prin sess_id st -> ());
+  pred_knowable = (fun tr prin sess_id st ->
+    match st with
+    | S cont -> 
+    serialize_wf_lemma state (is_knowable_by (principal_label prin) tr) st
+    | S2 _ n ->         serialize_wf_lemma state (is_knowable_by (principal_label prin) tr) st
+    );
+}
