Makefile
@@ -1,5 +1,5 @@
 # DY_HOME ?= ../../..
 
-EXAMPLES = nsl_pk_no_events_lookup TwoMessageP Online
+EXAMPLES = nsl_pk_no_events_lookup TwoMessageP Online Online_with_secrecy
 EXAMPLE_DIRS = dy-extensions $(addprefix examples/, $(EXAMPLES))
 include $(DY_HOME)/Makefile
